CollapsingTowers/TwoLvLBasic/StagingConsistency/Defs.lean
@@ -1,0 +1,2 @@
+import CollapsingTowers.TwoLvLBasic.StagingConsistency.ConsisHead
+import CollapsingTowers.TwoLvLBasic.StagingConsistency.Consistency
